implemented relative indices and worked on hoare_compose

HoareVerification/machine.lean
@@ -1,3 +1,4 @@
+
 /-
 
 A register machine is sequence of instructions of the form
@@ -13,4 +14,180 @@ We also add
 
   SET (r,v) : SET the value of register r to v
 
---/
+In Lean, we can define an inductive type to capture these rules syntactically.
+
+-/
+
+/-
+# TYPES
+-/
+
+namespace RM
+
+structure State where
+  pc : Int
+  mem : Nat → Nat
+
+def init : State := ⟨ 0, λ _ => 0 ⟩
+
+abbrev Action := State → State
+abbrev Program := List Action
+
+/-
+# INSTRUCTIONS
+-/
+/- Let's redo these so that indexes are relative. O is current instruction, 1 is one before, -1 is one behind, ect. -/
+@[simp]
+def set (r val : Nat) : Action := λ s => ⟨
+  s.pc+1,
+  λ x => if x = r then val else s.mem x
+⟩
+
+@[simp]
+def dec (r : Nat) : Action := λ s => ⟨
+  s.pc+1,
+  λ x => if x = r then s.mem x - 1 else s.mem x
+⟩
+
+@[simp]
+def jz (r : Nat) (loc : Int) : Action := λ s =>  ⟨
+  if s.mem r = 0 then s.pc + loc else s.pc+1,
+  s.mem
+⟩
+
+@[simp]
+def goto (loc : Int) : Action := λ s => ⟨
+  s.pc + loc,
+  s.mem
+  ⟩
+
+@[simp]
+def inc (r : Nat) : Action := λ s => ⟨
+  s.pc+1,
+  λ x => if x = r then s.mem x + 1 else s.mem x
+⟩
+
+@[simp]
+def clr (r : Nat) : Action := λ s => ⟨
+  s.pc+1,
+  λ x => if x = r then 0 else s.mem x
+⟩
+
+@[simp]
+def cpy (rj rk : Nat) : Action := λ s => ⟨
+  s.pc+1,
+  λ x => if x = rk then s.mem rj else s.mem x
+⟩
+
+@[simp]
+def je (rj rk : Nat) (z : Int) : Action := λ s => ⟨
+  if s.mem rj = s.mem rk then s.pc + z else s.pc + 1,
+  s.mem
+⟩
+
+
+/-
+# PROGRAMS
+-/
+
+def step (p : Program) : Action := λ s =>
+  if h : s.pc < p.length ∧ s.pc >= 0
+  then p[s.pc.toNat] s
+  else s
+
+def run (p : Program) (numsteps : Nat) : Action := λ s =>
+  match numsteps with
+  | Nat.zero => s
+  | Nat.succ k => run p k (step p s)
+
+
+
+def simple : Program := [
+  set 1 5,
+  dec 1,
+  goto (-1)
+
+]
+
+#eval (run simple 5 init).mem 1
+
+def set_mul : Program := [
+  -- Set initial values
+  set 1 5,
+  set 2 5,
+  -- incr r3 and r4
+  inc 3,
+  inc 4,
+  -- Check to see if r3 = r2. If so, reset, if not, inc again
+  je 2 3 2,
+  goto (-3),
+  -- reset
+  dec 1,
+  set 3 0,
+  -- Check if we're done, if not, loop.
+  jz 1 2,
+  goto (-7)
+]
+
+#eval (run set_mul 1000 init ).mem 4
+
+/-
+# HOARE LOGIC
+-/
+
+def Hoare (P : State → Prop)
+          (T : State → State)
+          (Q : State → Prop) :=
+  ∀ s, P s → Q (T s)
+
+def comp (P₁ P₂ : Program) : Program := P₁.append P₂
+
+
+theorem run_comp (P₁ P₂ : Program) (n : Nat) (a b : Fin n) (s : State) :
+run P₂ b (run P₁ a s) = run (P₁ ++ P₂) (a + b) s := by
+sorry
+
+
+
+
+/- Running program P₁ a times and then running P₂ b times is the same as running (comp P₁ P₂) a + b times. -/
+theorem hoare_compose
+  {P R Q: State → Prop}
+  {P₁ P₂ : Program}
+  {n : Nat}
+  {a b : Fin n}
+  : (Hoare P (run P₁ a) Q ∧ Hoare Q (run P₂ b) R) →
+  Hoare P (run (comp P₁ P₂) (a + b) ) R := by
+    unfold comp Hoare
+    intro ⟨ hq , hr ⟩ s hps
+    let s1 := run P₁ a s
+    have q_proof : Q s1 := hq s hps -- Both sides equal to Q s
+    let x := hr s1 q_proof
+    have run_comp : run P₂ b s1 = run (List.append P₁ P₂) (a + b) s := by
+
+      unfold s1 run
+      split
+      case _ h =>
+        . split
+          . case _ hab =>
+            rw[h] at hab
+            have ha : a = Nat.zero := by exact hab
+            unfold run
+            rw[ha]
+          . case _ k hab =>
+            rw[h] at hab
+            have ha : a = k.succ := by exact hab
+            . sorry
+      . case _ n h =>
+        . split
+          . case _ n h => sorry
+          . case _ n h => sorry
+
+
+    sorry
+
+
+
+
+
+theorem Videep : (True = True) := by rfl
